lean: implement Leibniz

lean4/Le/Basic.lean
@@ -1,1 +1,27 @@
+import Mathlib.Data.Nat.Basic
+import Lean
+
 def hello := "world"
+
+open Nat
+
+def fib (n : ℕ) : ℕ :=
+  match n with
+  | zero => 0
+  | succ zero => 1
+  | succ (succ n₂) => fib (n₂ + 1) + fib n₂
+
+-- #eval fib 0
+-- #eval fib 1
+-- #eval fib 2
+-- #eval fib 3
+-- #eval fib 4
+-- #eval fib 5
+
+lemma fib_is_fib (n : ℕ) : fib (succ (succ n)) = fib (succ n) + fib n := by
+  rw [fib]
+
+def leibniz (n: ℕ) (sum: Float) : Float :=
+  match n with
+  | 0 => sum
+  | succ n' =>  let k := (n * 4).toFloat; leibniz n' (sum + 8.0 / ((k - 1.0) * (k - 3.0)))
